soundness theorems for failure and join

ParserCombinators/Gen.lean
@@ -11,7 +11,7 @@ import ParserCombinators.Lemmas
 namespace Gen
 
 universe u
-variable {α ν : Type u} {μ : Type u → Type u} [Monad μ] [SemilatticeAlt μ] [Traversable μ] [BEq α] [DecidableEq α] [DecidableEq ν] [Hashable ν]
+variable {α ν : Type u} {μ : Type u → Type u} [Monad μ] [SemilatticeAlt μ] [Traversable μ] [BEq α] [DecidableEq α] [DecidableEq ν] [Hashable ν] [Fintype ν]
 
 open CFG
 open ParseTree
@@ -38,19 +38,23 @@ def gen' (cfg : @CFG α ν) (recur : ν → ParserM (tag := tag cfg) α μ (Pars
     pure $ ParseTree.Node n rule children
   ((cfg.rules n).attach.map parseRule).foldl ParserM.instMaxOfTraversableOfDecidableEq.max ⊥
 
-def gen (cfg : @CFG α ν) : ℕ → ν → ParserM (tag := tag cfg) α μ (ParseTree cfg) := withFuel' $ gen' cfg
+def gen (cfg : @CFG α ν) : ν → ParserM (tag := tag cfg) α μ (ParseTree cfg) := memoize (g := gen' cfg)
 
 -- TODO(maemre): correctness theorem (by injecting validity proofs above)
 -- TODO(maemre): correctness theorem (sound/complete)
 
-abbrev sound (cfg : @CFG α ν) [Membership (ParseTree cfg) (μ (ParseTree cfg))]
-  (n : ν) (p : ParserM (tag := tag cfg) α μ (ParseTree cfg)) (input : Array α)
-  := ∀ tree ∈ (runParser p input).1[0]?.getD ⊥, tree.Valid ∧ tree.root = Symbol.nonterm n
---
--- abbrev complete (cfg : @CFG α ν) [Membership (ParseTree cfg) (μ (ParseTree cfg))] (n : ν) (p : Parser (tag := tag cfg) α μ (ParseTree cfg)) (input : Array α)
---   (h : cfg.derives [Symbol.nonterm n] (input.toList.map Symbol.term))
---   := ∃ tree, tree ∈ (runParser p input).1[(0 : Int)]?.getD failure
+-- NOTE: We are proving these for Lists, we can later on generalize it to
+-- other "sensible" collections that preserve parts of a list.
 
+abbrev sound (cfg : @CFG α ν)
+  (n : ν) (p : ParserM (tag := tag cfg) α List (ParseTree cfg)) (input : Array α)
+  := ∀ tree ∈ (runParser p input).1.getD 0 ⊥, tree.Valid ∧ tree.root = Symbol.nonterm n
+
+abbrev complete (cfg : @CFG α ν) (n : ν) (p : ParserM (tag := tag cfg) α List (ParseTree cfg)) (input : Array α)
+  (h : cfg.derives [Symbol.nonterm n] (input.toList.map Symbol.term))
+  := ∃ tree, tree ∈ (runParser p input).1[0]?.getD ⊥
+
+omit [Fintype ν] in
 lemma failure_empty (cfg : @CFG α ν): (runParser (tag := tag cfg) (⊥ : ParserM α μ (ParseTree cfg)) input).1.isEmpty := by
   simp [Bot.bot, runParser, ReaderT.run, MStateT.run, ParserM.lift, ParserM.lower]
   unfold Parser.failure Parser.bind Bind.bind
@@ -69,11 +73,49 @@ lemma failure_empty (cfg : @CFG α ν): (runParser (tag := tag cfg) (⊥ : Parse
     whnf
   simp
 
--- theorem failure_sound (cfg : @CFG α ν) [Membership (ParseTree cfg) (μ (ParseTree cfg))] (n : ν) (input : Array α) : sound (μ := μ) cfg n failure input
---   := by
---   unfold sound
---   intro tree h
---   simp [Std.HashMap.getElem?_of_isEmpty, failure_empty] at h
---   sorry -- add a new type-class
+omit [Monad μ] [SemilatticeAlt μ] [Traversable μ] [Fintype ν] in
+theorem failure_sound (cfg : @CFG α ν) (n : ν) (input : Array α) : sound cfg n ⊥ input
+  := by
+  unfold sound
+  intro tree
+  simp [Std.HashMap.getD_of_isEmpty, failure_empty]
+  simp [Bot.bot, SemilatticeAlt.failure]
+
+omit [Monad μ] [SemilatticeAlt μ] [Traversable μ] [Fintype ν] in
+/-- The join operation on lists preserves soundness. -/
+theorem sound_of_sup_sound (cfg : @CFG α ν) (n : ν) (p q : ParserM (tag := tag cfg) α List (ParseTree cfg)) (input : Array α)
+  (h_p : sound cfg n p input) (h_q : sound cfg n q input) : sound cfg n (p ⊔ q) input
+  := by
+  unfold sound at *
+  intro tree h_mem
+  -- Extract subset relationships to use with h_mem
+  have h := runParser_sup_eq_sup_runParser p q input
+  have h' := Std.HashMap.EquivQuot.getD_eq (s := SemilatticeAlt.setoid) (k := 0) (fallback := ⊥) h
+  simp [SemilatticeAlt.setoid, List.memSetoid] at h'
+  dsimp [Subset, List.Subset] at *
+  replace h_mem := @h'.1 tree h_mem
+  dsimp [Max.max] at h_mem
+  by_cases h_p_contains_0 : 0 ∈ (runParser p input).1
+  · by_cases h_q_contains_0 : 0 ∈ (runParser q input).1
+    · rw [<- Std.HashMap.getElem_eq_getD] at h_p <;> simp_all
+      rw [<- Std.HashMap.getElem_eq_getD] at h_q <;> try simp_all
+      -- The explicit application is for providing the Semilatticeoid instance.
+      have h' := Std.HashMap.unionSup_getD_both (s := SemilatticeAlt.setoid) (semi := List.instSemilatticeAlt.instSemilatticeoidInstSetoid) h_p_contains_0 h_q_contains_0
+      simp [SemilatticeAlt.setoid, List.memSetoid, Subset, List.Subset] at h'
+      replace h_mem := @h'.1 tree h_mem
+      simp [Max.max, SemilatticeAlt.orElse] at h_mem
+      cases h_mem <;> rename_i h_mem
+      · exact h_p tree h_mem
+      · exact h_q tree h_mem
+    · have h' := Std.HashMap.unionSup_getD_of_right_not_contains (s := SemilatticeAlt.setoid) (semi := List.instSemilatticeAlt.instSemilatticeoidInstSetoid) (fallback := ⊥) (runParser p input).1 (runParser q input).1 h_q_contains_0
+      simp [SemilatticeAlt.setoid, List.memSetoid, Subset, List.Subset] at h'
+      replace h_mem := @h'.1 tree h_mem
+      exact h_p tree h_mem
+  · have h' := Std.HashMap.unionSup_getD_of_not_contains (s := SemilatticeAlt.setoid) (semi := List.instSemilatticeAlt.instSemilatticeoidInstSetoid) (fallback := ⊥) (runParser p input).1 (runParser q input).1 h_p_contains_0
+    simp [SemilatticeAlt.setoid, List.memSetoid, Subset, List.Subset] at h'
+    replace h_mem := @h'.1 tree h_mem
+    by_cases h_q_contains_0 : 0 ∈ (runParser q input).1
+    · exact h_q tree h_mem
+    · simp_all
 
 end Gen
